Inserters/Xor.dfy
@@ -1,0 +1,36 @@
+module Inserters.XOr{
+
+  import opened Circ
+  import opened Utils
+  import opened ConservedSubcircuit
+  import opened MapFunction
+  import opened Inserters_Binary
+  import opened Modifiers.SwitchUF
+
+  const XorUFConst := UpdateFunction(
+    2, 1, 0,
+    (si: SI) requires |si.inputs| == 2 && |si.state| == 0 =>
+      SO([Xor(si.inputs[0], si.inputs[1])], []))
+
+  opaque function XorUF(): (r: UpdateFunction)
+    ensures r.Valid()
+    ensures r.input_width == 2
+    ensures r.output_width == 1
+    ensures r.state_width == 0
+  {
+    reveal UpdateFunction.Valid();
+    XorUFConst
+  }
+
+  opaque function XorInserter(): (z: ScufInserter)
+    ensures z.Valid()
+    ensures z.uf == XorUF()
+  {
+    var z_binary := BinaryInserter(CXor);
+    reveal UpdateFunctionsEquiv();
+    reveal XorUF();
+    var z := SwitchUFModifier(z_binary, XorUF());
+    z
+  }
+
+}
